dafny/src/main.dfy
@@ -1,0 +1,12 @@
+
+include "libs/math.dfy"
+
+import opened Math2
+
+method Main() {
+    var arr := new int[5] [1, 2, 4, 7, 9];
+    var key := 1;
+    var index :nat := BinarySearch2(arr, key);
+    print index;
+    print "\n";
+}
