dafny/doc/DAFNY.md
@@ -1,0 +1,35 @@
+
+
+
+
+```dafny
+
+    predicate sorted2(a: array<int>)
+    reads a {
+        forall j, k :: 0 <= j < k < a.Length ==> a[j] <= a[k]
+    }
+
+    method BinarySearch2(a: array<int>, key: int) returns (index: int)
+    requires sorted2(a)
+    ensures 0 <= index ==> index < a.Length && a[index] == key
+    ensures index < 0 ==> forall k :: 0 <= k < a.Length ==> a[k] != key {
+
+    var low, high := 0, a.Length;
+        while low < high
+        invariant 0 <= low <= high <= a.Length
+        invariant forall i ::
+        0 <= i < a.Length && !(low <= i < high) ==> a[i] != key {
+            var mid := (low + high) / 2;
+            if a[mid] < key {
+                low := mid + 1;
+            }
+            else if key < a[mid] {
+                high := mid;
+            }
+            else {
+                return mid;
+            }
+        }
+        return -1;
+    }
+```
